하....이제 'Uniqueness' 에 대한 식을 만들어야 할 듯

src/common/Nemonuri.Bijective.IndexMap.fst
@@ -2,32 +2,82 @@ module Nemonuri.Bijective.IndexMap
 
 module I = FStar.IntegerIntervals
 module ISet = Nemonuri.IndexSet
+open Nemonuri.IndexMap { count, last_key, first_key, key_t, contained_data_t,
+                         ensured_data_t, max_key,
+                         key_value, is_empty,
+                         interval_does_not_contain_value }
+open Nemonuri.IndexMap.Unique
 module IMap = Nemonuri.IndexMap
 module Seq = FStar.Seq.Base
 module List = FStar.List.Tot
+open FStar.Bijection { (=~) }
 module B = FStar.Bijection
 
+let interval_is_bijective (#data_t:eqtype) (m:IMap.t data_t) (min:key_t m) (imax:key_t m) =
+  forall (x:key_t m). (I.interval_condition min (imax+1) x) ==>
+    ((min = imax) <==> (IMap.select m min = IMap.select m imax))
+
 let bijective_index_map_predicate (#data_t:eqtype) (m:IMap.t data_t) =
-  m |> IMap.to_seq |> Seq.seq_to_list |> List.noRepeats
+  forall (x:contained_data_t m). (unique_data_predicate m x)
+  //m |> IMap.to_seq |> Seq.seq_to_list |> List.noRepeats
+
+(*
+let lemma_bijective_index_map_predicate (#data_t:eqtype) (m:IMap.ensured_t data_t)
+  : Lemma ((interval_is_bijective m 0 (max_key m)) <==> (bijective_index_map_predicate m))
+  =
+  ()
+*)
+
+(*
+private let rec is_bijective_agg' 
+  (#data_t:eqtype) (m:IMap.t data_t) 
+  (asc_select_key:key_t m) (des_compare_key:key_t m{des_compare_key < asc_select_key})
+  =
+*)
+
 
 type t (data_t:eqtype) = x:IMap.t data_t{bijective_index_map_predicate x}
 
-//let index_of 
+type ensured_t (data_t:eqtype) = x:t data_t{not (is_empty x)}
 
-//let lemma_bijective_index_map #data_t (m:t data_t)
-//  : Lemma
+let lemma_key #data_t (m:t data_t) (key:key_t m)
+  : Lemma (unique_key_predicate m key) =
+  ()
+
+let select #data_t (m:t data_t) (key:unique_key_t m) : Tot (unique_data_t m) = IMap.select m key
+let unique_key #data_t (m:t data_t) (v:unique_data_t m) : Tot (unique_key_t m) = IMap.first_key m v
+
+
+let empty (#data_t:eqtype) (fb:data_t) : Tot (t data_t) = IMap.empty fb
+
+let fresh_data_predicate #data_t (m:t data_t) (v:ensured_data_t m) : Tot bool = not (IMap.contains_value m v)
+type fresh_data_t #data_t (m:t data_t) = x:ensured_data_t m{fresh_data_predicate m x}
 
 
 
 
-type bijection_t #data_t (m:t data_t) = B.bijection (IMap.key_t m) (IMap.contained_data_t m)
-
-
+//let lemma_push_fresh_data_unique #data_t (m:t data_t) (v:fresh_data_t m)
 
 (*
-let to_bijection #data_t (m:t data_t)
-  : Tot (bijection_t m) =
-  {
-    right = 
-  }
+let pop #data_t (m:ensured_t data_t) : Tot ((t data_t) & (key_value data_t)) =
+  let ( m2, kv ) = IMap.pop m in
+  ( m2, kv )
 *)
+
+let push #data_t (m:t data_t) (v:fresh_data_t m) 
+  : Tot (t data_t) = 
+  let next_m = IMap.push m v in
+  assert (interval_does_not_contain_value next_m v 0 (count m));
+  assert (~(interval_does_not_contain_value next_m v 0 (count next_m)));
+  assert ((last_key next_m v) = (first_key next_m v));
+  assert (unique_data_predicate next_m v);
+  //assume (IMap.first_key next_m v = IMap.max_key next_m);
+  //assume (IMap.last_key next_m v = IMap.max_key next_m);
+  //assert (IMap.first_key next_m v = IMap.last_key next_m v);
+  //assume (forall (x:key_t m). (unique_key_predicate next_m x));
+  //assert (unique_data_predicate next_m v);
+  assume (bijective_index_map_predicate next_m);
+  next_m
+  
+
+
