src/common/Nemonuri.Bijective.IndexMap.Bijection.fst
@@ -1,0 +1,23 @@
+module Nemonuri.Bijective.IndexMap.Bijection
+
+open Nemonuri.Bijective.IndexMap
+open Nemonuri.IndexMap { key_t, unique_data_predicate, unique_data_t, contained_data_t,
+                         unique_key_predicate, unique_key_t, ensured_data_t }
+open FStar.Bijection { (=~) }
+module B = FStar.Bijection
+
+let lemma_select_and_unique_key #data_t (m:t data_t) (key:unique_key_t m)
+  : Lemma (unique_key m (select m key) == key) = ()
+let lemma_unique_key_and_select #data_t (m:t data_t) (v:unique_data_t m)
+  : Lemma (select m (unique_key m v) == v) = ()
+
+type bijection_t #data_t (m:t data_t) = (unique_key_t m) =~ (unique_data_t m)
+
+let to_bijection #data_t (m:t data_t)
+  : Tot (bijection_t m) =
+  {
+    right = select m;
+    left = unique_key m;
+    left_right = lemma_select_and_unique_key m;
+    right_left = lemma_unique_key_and_select m;
+  }
