src/common/Nemonuri.IndexMap.Unique.fst
@@ -1,0 +1,39 @@
+module Nemonuri.IndexMap.Unique
+
+open Nemonuri.IndexMap
+module Cl = FStar.Classical
+
+let unique_data_predicate (#data_t:eqtype) (m:t data_t) (v:contained_data_t m) : Tot bool =
+  (last_key m v) = (first_key m v)
+
+type unique_data_t (#data_t:eqtype) (m:t data_t) = x:contained_data_t m{unique_data_predicate m x}
+
+//let lemma_unique_data2 (#data_t:eqtype) (m:t data_t) (v:unique_data_t m)
+//  : Lemma ()
+
+let lemma_unique_data (#data_t:eqtype) (m:t data_t) (k:key_t m) (v:contained_data_t m)
+  : Lemma ((unique_data_predicate m v) ==> ((v = select m k) <==> (last_key m v = k)))
+  =
+  match (unique_data_predicate m v) with | false -> () | true ->
+  let uk = last_key m v in
+  assert (~(interval_does_not_contain_value m v 0 (count m)));
+  assert (interval_does_not_contain_value m v (uk+1) (count m));
+  assert (interval_does_not_contain_value m v 0 uk);
+  assert (v = select m uk)
+  (*
+  let pl = (v = select m k) in
+  let pr = (last_key m v = k) in
+  let lemma_l_to_r' () : Lemma (requires pl) (ensures pr) =
+    assert (uk = k)
+  in
+  let lemma_r_to_l' () : Lemma (requires pr) (ensures pl) =
+     ()
+  in
+  Cl.move_requires lemma_l_to_r' ();
+  Cl.move_requires lemma_r_to_l' ()
+  *)
+
+let unique_key_predicate (#data_t:eqtype) (m:t data_t) (key:key_t m) : Tot bool =
+  select m key |> unique_data_predicate m
+
+type unique_key_t (#data_t:eqtype) (m:t data_t) = x:key_t m{unique_key_predicate m x}
